\section*{Laplace Transform}
\subsection*{Definition}
\begin{align*}
    \func{f}[t] &= \frac{1}{2 \pi j} \intidef{\func{F}[s] e^{st}}[s] \\
    \func{F}[s] &= \intdef{0}{\infty}{\func{f}[t] e^{-st}}{t}
\end{align*}

\subsection*{Special Cases}
\begin{align*}
    \laplace{e^{pt}} &= \frac{1}{s-p} \forall p \in \mathbb{C} \\
    \laplace{Ae^{at}\cos{bt+\psi}} &= \frac{C}{s-p}+\frac{\overline{C}}{s-\overline{p}}, C = \frac{A}{2}e^{j\psi} \\
    \laplace{c} &= \frac{c}{s} \forall c \in \mathbb{C}
\end{align*}

\subsection*{Properties}
\begin{align*}
    \laplace{\func{f_1}[t] + \func{f_2}[t]} &= \func{F_1}[s]+\func{F_2}[s] \\
    \laplace{\func{f_1}[t]\func{f_2}[t]} &\neq \func{F_1}[s]\func{F_2}[s] \\
    \laplace{\func{\dot{f}}[t]} &= s \func{F}[s] - \func{f}[0] \\
    \laplace{\func{f^{(k)}}[t]} &= s^{k} \func{F}[s] - \sum_{i=1}^{k} s^{i-1}\func{f^{(k-i)}}[0] \\
    \laplace{t \func{f}[t]} &= -\deriv{s}{\func{F}[s]} \\
    \laplace{t e^{pt}} &= -\deriv{s}{\frac{1}{s-p}} \\
    \laplace{t^{k} e^{pt}} &= \frac{k!}{{(s-p)}^{k+1}}
\end{align*}

\subsection*{Usage}
\begin{align*}
    \func{r}[s]\func{Y}[s]-\func{c}[s] &= \func{q}[s]\func{U}[s]-\func{b}[s] \\
    \func{r}[s] &= \alpha_n s^n + \cdots + \alpha_1 s + \alpha_0 \\
    \func{q}[s] &= \beta_m s^m + \cdots + \beta_1 s + \beta_0 \\
    \func{c}[s] &= n-1 \text{ order poly from IC on } \func{y}[t] \\
    \func{b}[s] &= m-1 \text{ order poly from IC on } \func{u}[t] \\
    \func{Y}[s] &= \func{G}[s]\func{U}[s]+\left[\frac{\func{c}[s]-\func{b}[s]}{\func{r}[s]}\right]
\end{align*}